src/HOL/IMPP/Natural.thy
@@ -111,7 +111,9 @@ done
 
 lemma evaln_evalc: "<c,s> -n-> t ==> <c,s> -c-> t"
 apply (erule evaln.induct)
-apply (tactic {* ALLGOALS (resolve_tac @{context} @{thms evalc.intros} THEN_ALL_NEW atac) *})
+apply (tactic {*
+  ALLGOALS (resolve_tac @{context} @{thms evalc.intros} THEN_ALL_NEW assume_tac @{context})
+*})
 done
 
 lemma Suc_le_D_lemma: "[| Suc n <= m'; (!!m. n <= m ==> P (Suc m)) |] ==> P m'"
@@ -137,11 +139,12 @@ done
 
 lemma evalc_evaln: "<c,s> -c-> t ==> ? n. <c,s> -n-> t"
 apply (erule evalc.induct)
-apply (tactic {* ALLGOALS (REPEAT o etac exE) *})
-apply (tactic {* TRYALL (EVERY' [dtac @{thm evaln_max2}, assume_tac @{context},
+apply (tactic {* ALLGOALS (REPEAT o eresolve_tac @{context} [exE]) *})
+apply (tactic {* TRYALL (EVERY' [dresolve_tac @{context} @{thms evaln_max2}, assume_tac @{context},
   REPEAT o eresolve_tac @{context} [exE, conjE]]) *})
 apply (tactic
-  {* ALLGOALS (rtac exI THEN' resolve_tac @{context} @{thms evaln.intros} THEN_ALL_NEW atac) *})
+  {* ALLGOALS (resolve_tac @{context} [exI] THEN'
+    resolve_tac @{context} @{thms evaln.intros} THEN_ALL_NEW assume_tac @{context}) *})
 done
 
 lemma eval_eq: "<c,s> -c-> t = (? n. <c,s> -n-> t)"
